coq: Add a ‘Show’ typeclass and a ‘derive_show’ tactic

coq/Common.v
@@ -1,7 +1,7 @@
 Require Import Coq.Lists.List Coq.Bool.Bool Coq.Strings.String.
 Require Export Coq.omega.Omega.
 Import ListNotations.
-Require Export Koika.EqDec Koika.Vect Koika.FiniteType.
+Require Export Koika.EqDec Koika.Vect Koika.FiniteType Koika.Show.
 
 (* https://coq-club.inria.narkive.com/HeWqgvKm/boolean-simplification *)
 Hint Rewrite
@@ -275,33 +275,6 @@ Section result_list_map.
                Success (b :: la)
     end.
 End result_list_map.
-
-Section string_of_nat.
-  Lemma digit_lt_base m {n} : not (m + n < m).
-  Proof.
-    red; intros; eapply Le.le_Sn_n; eauto using Le.le_trans, Plus.le_plus_l.
-  Qed.
-
-  Definition string_of_base10_digit (n: {n | n < 10}) :=
-    match n with
-    | exist _ 0 _ => "0" | exist _ 1 _ => "1" | exist _ 2 _ => "2" | exist _ 3 _ => "3" | exist _ 4 _ => "4"
-    | exist _ 5 _ => "5" | exist _ 6 _ => "6" | exist _ 7 _ => "7" | exist _ 8 _ => "8" | exist _ 9 _ => "9"
-    | exist _ n pr => False_rect _ (digit_lt_base 10 pr)
-    end%string.
-
-  Fixpoint string_of_nat_rec (fuel: nat) (n: nat) :=
-    match fuel with
-    | O => ""%string
-    | S fuel =>
-      match (Compare_dec.lt_dec n 10) with
-      | left pr  => string_of_base10_digit (exist _ n pr)
-      | right pr => append (string_of_nat_rec fuel (PeanoNat.Nat.div n 10)) (string_of_nat_rec fuel (PeanoNat.Nat.modulo n 10))
-      end
-    end.
-
-  Definition string_of_nat (n: nat) :=
-    string_of_nat_rec (S n) n.
-End string_of_nat.
 
 Axiom __magic__ : forall {A}, A.
 
