coq/DeriveShow.v
@@ -1,0 +1,105 @@
+Require Import Koika.Show.
+
+Require Koika.IdentParsing.
+Require Import Ltac2.Ltac2.
+
+Import Ltac2.Init.
+Import Ltac2.Notations.
+
+Module Internals.
+  Import Coq.Lists.List.ListNotations.
+  Import IdentParsing.Unsafe.
+  Import IdentParsing.
+
+  Ltac2 Type exn ::= [ NotAConstructor (constr) ].
+
+  Ltac2 rec list_map fn l :=
+    match l with
+    | [] => []
+    | h :: t => fn h :: list_map fn t
+    end.
+
+  Ltac2 rec coq_list_of_list type fn ls :=
+    match ls with
+    | [] => constr:(@List.nil $type)
+    | h :: t =>
+      let ch := fn h in
+      let ct := coq_list_of_list type fn t in
+      constr:($ch :: $ct)
+    end.
+
+  Ltac2 path_of_constructor c :=
+    match Constr.Unsafe.kind c with
+    | Constr.Unsafe.Constructor cstr _ =>
+      let path := Env.path (Std.ConstructRef cstr) in
+      coq_list_of_list constr:(String.string) coq_string_of_ident path
+    | _ => Control.throw (NotAConstructor c)
+    end.
+
+  Ltac2 unpack_app c :=
+    let rec loop acc c :=
+        match! c with
+        | ?f ?x => loop (x :: acc) f
+        | ?x => x, acc
+        end in
+    loop [] c.
+
+  Definition blocked (A: Type) := A.
+
+  Ltac not_blocked t :=
+    lazymatch t with
+    | blocked _ => fail
+    | _ => idtac
+    end.
+
+  Inductive Tracked {A} (x: A) := Track.
+
+  Definition type_of {A} (a: A) := A.
+
+  Fixpoint butlast {A} (l: list A) :=
+    match l with
+    | [] => []
+    | [x] => [x]
+    | hd :: tl => butlast tl
+    end.
+
+  Ltac2 derive_show_begin () :=
+    ltac1:(match goal with
+           | [  |- Show ?type ] =>
+             econstructor;
+               let term := fresh in
+               intro term; pose proof (@Track type term); destruct term
+           end).
+
+  Ltac2 derive_show_recurse arg :=
+    (* let instance := constr:(ltac:(typeclasses eauto) : Show (type_of $arg)) in *)
+    constr:(show $arg).
+
+  Ltac2 rec derive_show_app () :=
+    lazy_match! goal with
+    | [ _: Tracked ?app |- _ ] =>
+      match unpack_app app with
+      | (hd, args) => let hd_path := path_of_constructor hd in
+                     let hd_str := constr:(String.concat "_" (butlast $hd_path)) in
+                     let arg_strs := coq_list_of_list constr:(String.string) derive_show_recurse args in
+                     let str := constr:(String.concat "_" ($hd_str :: $arg_strs)) in
+                     let str := compute str in
+                     exact $str
+      end
+    end.
+
+  Ltac2 rec derive_show () :=
+    Control.enter derive_show_begin; Control.enter derive_show_app.
+
+  Hint Extern 2 (Show _) => ltac2:(derive_show ()) : typeclass_instances.
+End Internals.
+
+Ltac derive_show :=
+  ltac2:(Control.enter Internals.derive_show).
+
+Module Examples.
+  Inductive x := X0 | X1 | X2.
+  Inductive y := Y0 (_: x) | Y1 .
+
+  Definition test (n: nat) : Show y := _.
+End Examples.
